Prove proper postcondition for Make coord server

src/program_proof/memkv/memkv_coord_definitions.v
@@ -3,7 +3,7 @@ From Goose.github_com.mit_pdos.gokv Require Import memkv.
 From Perennial.program_proof.lockservice Require Import rpc.
 From Perennial.program_proof.memkv Require Import common_proof memkv_shard_definitions.
 
-Section memkv_coord_definitions.
+Section memkv_global_coord_definitions.
 
 (* TODO: should it be heap_globalG or heapG? *)
 (* I think the former because it is sent from a coord server to a client *)
@@ -12,6 +12,20 @@ Context `{!dist_lifting.heap_globalG Σ, rpcG Σ ShardReplyC, rpcregG Σ, kvMapG
 Definition all_are_shard_servers (s:list u64) γkv : iProp Σ :=
   ∀ sid host, ⌜s !! sid = Some host⌝ →
               (∃ γ, is_shard_server host γ ∗ ⌜γ.(kv_gn) = γkv⌝)
+.
+
+End memkv_global_coord_definitions.
+
+
+Section memkv_coord_definitions.
+
+Context `{!heapG Σ, rpcG Σ ShardReplyC, rpcregG Σ, kvMapG Σ}.
+
+Definition own_ShardClerkSet (s:loc) (γkv:gname) : iProp Σ :=
+  ∃ (cls_ptr:loc) (clsM:gmap u64 loc),
+  "Hcls" ∷ s ↦[ShardClerkSet :: "cls"] #cls_ptr ∗
+  "HclsMap" ∷ is_map cls_ptr 1 clsM ∗
+  "HclsOwn" ∷ [∗ map] host ↦ cl_ptr ∈ clsM, own_MemKVShardClerk cl_ptr γkv
 .
 
 End memkv_coord_definitions.
