src/ShouldBuild.v
@@ -31,7 +31,8 @@ From Perennial.program_proof.lockservice Require
 (* In-memory sharded KV system *)
 From Perennial.program_proof.memkv Require
      rpc_proof
-     memkv_clerk_proof memkv_shard_start_proof memkv_shard_make_proof closed.
+     memkv_clerk_proof memkv_shard_start_proof memkv_shard_make_proof memkv_coord_make_proof
+     closed.
 
 From Perennial.goose_lang Require
      ffi.append_log_ffi.
